Instances/IsBool/Boolean.v
@@ -4,31 +4,35 @@ Require Import Language.Statements.
 Require Import Types.State.
 Require Import Types.Stores.
 Require Import Types.Result.
+Require Import Instances.Monad.
 
 Definition ensure_bool (v : cvalue) : State bool :=
-  fun st => match v with
-            | VBool b => returnR b st
-            | _ => crashed 
-            end.
+  match v with
+  | VBool b => Just _ (returnM b)
+  | _ => None _
+  end.
 
 Definition build_boolean (b : bool) : State cvalue :=
-  returnM (VBool b).
+  Just _ (returnM (VBool b)).
 
 Definition extract_boolean (b : bool) : State bool :=
-  returnM b.
+  Just _ (returnM b).
 
-Definition andbM (b c : bool) : State bool := returnM (andb b c).
+Definition andbM (b c : bool) : State bool := 
+  Just _ (returnM (andb b c)).
 
-Definition negbM (b : bool) : State bool := returnM (negb b).
+Definition negbM (b : bool) : State bool := 
+  Just _ (returnM (negb b)).
 
 Definition eval_if {A} (b : bool) (st1 st2 : State A) : State A :=
   if b then st1 else st2.
+
 
 Instance boolean_type : IsBool State cvalue bool :=
 {
   ensure_bool := ensure_bool;
   build_bool := build_boolean;
-  extract_bool := fun b => returnM b;
+  extract_bool := extract_boolean;
   and_op := andbM;
   neg_op := negbM;
   if_op := eval_if;
