Instances/Monad.v
@@ -1,0 +1,95 @@
+Require Import Classes.Monad.
+Require Import Language.Statements.
+Require Import Types.Maps.
+
+Section Maybe.
+  Inductive Maybe (A : Type) : Type :=
+    | Just : A -> Maybe A
+    | None : Maybe A.
+  Arguments Just {_}.
+  Arguments None {_}.
+  Check Just.
+
+  Definition return_maybe {A : Type} (a : A) : Maybe A :=
+    Just a.
+  Arguments return_maybe [_].
+
+  Definition bind_maybe {A B : Type} 
+    (m : Maybe A) (k : A -> Maybe B) : Maybe B :=
+    match m with
+    | None => None
+    | Just a => k a
+    end.
+  Arguments bind_maybe [_ _].
+
+  Global Instance monad_maybe : Monad Maybe :=
+  {
+    returnM := return_maybe;
+    bindM := bind_maybe;
+  }.
+
+End Maybe.
+
+Section AbstractMaybe.
+  Inductive AbstractMaybe (A : Type) : Type :=
+    | JustA : A -> AbstractMaybe A
+    | JustOrNoneA : A -> AbstractMaybe A
+    | NoneA : AbstractMaybe A.
+  Arguments JustA {_}.
+  Arguments JustOrNoneA {_}.
+  Arguments NoneA {_}.
+
+  Definition return_maybeA {A : Type} (a : A) : AbstractMaybe A :=
+    JustA a.
+  Arguments return_maybeA [_].
+
+  Definition bind_maybeA {A B : Type}
+    (m : AbstractMaybe A) (k : A -> AbstractMaybe B) : AbstractMaybe B :=
+    match m with
+    | NoneA => NoneA
+    | JustA a => k a
+    | JustOrNoneA a => match (k a) with
+                       | NoneA => NoneA
+                       | JustA b => JustOrNoneA b
+                       | JustOrNoneA b => JustOrNoneA b
+                       end
+    end.
+  Arguments bind_maybeA [_].
+
+  Global Instance monad_abstract_maybe : Monad AbstractMaybe :=
+  {
+    returnM := return_maybeA;
+    bindM := bind_maybeA;
+  }.
+End AbstractMaybe.
+
+Section State.
+
+  Definition state (S A : Type) := S -> (A * S).
+  Definition return_state {S A : Type} (a : A) : state S A :=
+    fun st => (a, st).
+  Arguments return_state {_} [_].
+
+(*Definition bind_state {A B : Type} (m : State A) (f : A -> State B) 
+    : State B :=
+  fun st => match m st with
+            | returnR x st' => f x st'
+            | crashed => crashed 
+            | exception st' => exception st'
+            end.*)
+  Definition bind_state {S A B : Type} 
+    (p : state S A) (k : A -> state S B) : state S B :=
+    fun st => match (p st) with
+              | (x, st') => k x st'
+              end.
+  Arguments bind_state {_} [_ _].
+
+  Global Instance monad_state : forall s, Monad (state s) :=
+  {
+    returnM := return_state;
+    bindM := bind_state;
+  }.
+End State.
+
+
+  
