Instances/Store/AbstractStore.v
@@ -5,6 +5,7 @@ Require Import Types.Maps.
 Require Import Types.Result.
 Require Import Types.State.
 Require Import Types.Stores.
+Require Import Instances.Monad.
 
 Definition abstract_store_top : abstract_store :=
   fun _ => VTop.
@@ -14,14 +15,15 @@ Definition abstract_store_join
     (ast1 ast2 : abstract_store) : abstract_store :=
   fun x => VTop.
 
-Definition abstract_store_get (x : string) : 
-  AbstractState avalue := 
-  fun st => returnRA (st x) st.
+Compute (AbstractState avalue).
+
+Definition abstract_store_get (x : string) : AbstractState avalue := 
+  JustA _ (fun st : (total_map avalue) => (st x, st)).
 
 Definition abstract_store_put 
   (x : string) (v : avalue) : 
   AbstractState unit :=
-  fun st => returnRA tt (t_update st x v).
+  JustA _ (fun st => (tt, (t_update st x v))).
 
 Instance store_abstract : Store AbstractState avalue := {
   get := abstract_store_get;
