Instances/Store/ConcreteStore.v
@@ -4,12 +4,13 @@ Require Import Classes.Store.
 Require Import Types.State.
 Require Import Types.Result.
 Require Import Types.Stores.
+Require Import Instances.Monad.
 
-Definition store_get (x : string) : State cvalue := fun st =>
-  returnR (st x) st.
+Definition store_get (x : string) : State cvalue := 
+  Just _ (fun st => (st x, st)).
 
 Definition store_put (x : string) (v : cvalue) : State unit := 
-  fun st => returnR tt (t_update st x v).
+  Just _ (fun st => (tt, (t_update st x v))).
 
 Instance store_concrete : Store State cvalue := {
   get := store_get;
